automata.v
@@ -2,7 +2,6 @@
 
 Require Import Utf8 Bool PeanoNat List Eqdep_dec.
 From larith Require Import tactics notations utilities order dfs.
-Import ListNotations.
 
 Record automaton (letter : Set) := Automaton {
   state  : Set;
